platform/Depl/Compile.v
@@ -1,0 +1,51 @@
+(** Compiling the deeply embedded programming language *)
+
+Require Import AutoSep Wrap.
+
+Require Import Depl.Logic Depl.Cancel Depl.AlgebraicDatatypes Depl.Statements.
+
+
+(** * Lowering DEPL expressions to Bedrock SPS expressions *)
+
+Definition exprC (e : expr) : rvalue' :=
+  match e with
+    | Var x => x
+    | Const w => w
+  end.
+(** The above looks like a bit of magic.  It's all in the coercions (from main Bedrock library). *)
+
+Theorem exprC_correct : forall specs P stn st xs V vs fE e e' res,
+  vars_ok fE V vs
+  -> exprD vs e = Some e'
+  -> exprV xs e
+  -> ~In "rp" xs
+  -> interp specs (![locals ("rp" :: xs) V res (Regs st Sp) * P] (stn, st))
+  -> exists w,
+    evalRvalue stn st (exprC e xs) = Some w
+    /\ Logic.exprD e' fE = Dyn w.
+Proof.
+  destruct e; simpl; intuition.
+
+  injection H0; clear H0; intros; subst; eauto.
+
+  assert (Hnone : evalInstrs stn st (IL.Assign Rv (variableSlot x xs) :: nil) <> None).
+  simp.
+  generalize dependent H0.
+  evaluate auto_ext.
+
+  assert (Hsome : forall st', evalInstrs stn st (IL.Assign Rv (variableSlot x xs) :: nil) = Some st'
+    -> Regs st' Rv = sel V x).
+  simp.
+  generalize dependent H0.
+  evaluate auto_ext; auto.
+
+  Transparent evalInstrs.
+  simpl in *.
+  Opaque evalInstrs.
+  match goal with
+    | [ |- exists x, ?X = _ /\ _ ] => destruct X; try tauto
+  end.
+  specialize (Hsome _ eq_refl); simpl in *.
+  rewrite rupd_eq in Hsome; subst.
+  eauto.
+Qed.
